\documentclass[12pt,a4paper]{report}
\usepackage[utf8]{inputenc}
\usepackage{amsmath}
\newcommand{\norm}[1]{\left\lVert#1\right\rVert}
\usepackage{amsfonts}
\usepackage{comment}
\usepackage{nicefrac}
\usepackage[margin=3.3cm]{geometry}
\usepackage{amssymb}
\usepackage{accents}
\usepackage{amsthm}
\usepackage[pdftex, pdfborderstyle={/S/U/W 0}]{hyperref}
\numberwithin{equation}{section}
\usepackage{commath}
\usepackage{graphicx}
%\usepackage[extreme]{savetrees}
\usepackage{bm}
\usepackage{indentfirst}
\usepackage{nicefrac}
\setcounter{tocdepth}{4}
\usepackage{fnpct}
\usepackage{centernot}

\usepackage{cool}
\Style{DSymb={\mathrm d},DShorten=true,IntegrateDifferentialDSymb=\mathrm{d}}

\usepackage{microtype}
\usepackage{cleveref}

\theoremstyle{definition}
\newtheorem{definition}{Definition}[section]
\usepackage{mathtools}
 
\theoremstyle{remark}
\newtheorem*{remark}{Remark}

\newtheorem{theorem}{Theorem}[section]
\newtheorem{corollary}{Corollary}[theorem]
\newtheorem{lemma}[theorem]{Lemma}

\usepackage{url}
\newcommand*{\defeq}{\stackrel{\text{def}}{=}}
\author{Jacopo Tissino}
\title{Notes on Calculus I}

\begin{document}

\maketitle

\chapter{Naïve set theory}

\section{Basic sets}

\begin{equation}
\mathbb{N} \subseteq \mathbb{Z} \subseteq \mathbb{Q} \subseteq \mathbb{R}, \qquad 0 \not \in \mathbb{N}
\end{equation}

\begin{equation}
\mathbb{R}^+ := \lbrace x \in \mathbb{R} : x>0 \rbrace
\end{equation}

\paragraph{Remarks}

\begin{itemize}
\item ``$\in$'' is for elements belonging to sets, ``$\subseteq$'' is for subsets
\item $\lbrace x \rbrace \neq x$: the first is a set with $x$ as its only element, and is called a ``singlet''
\item $\subsetneq$  means ``is a subset of, but not equal to''
\item the elements of $\mathcal{P}(A)$ are precisely all the subsets of $A$
\item $\sharp A$ is the cardinality of $A$
\item $\sharp \mathcal{P} (A) = 2^{\sharp A}$
\end{itemize}

The naïve definitions of $A \cup B$, $A \cap B$, $A \smallsetminus B$ are given.

\paragraph{Properties}

\begin{itemize}
\item $A = (A \cap B ) \cup (A \smallsetminus B)$
\item $(A \cap B) \cap (A \smallsetminus B) = \emptyset$
\item $C \cap (A \cup B) = (C \cap A) \cup (C \cap B)$
\item $C \cup (A \cap B) = (C \cup A) \cap (C \cup B)$
\end{itemize}

\paragraph{Complement}

\begin{definition}
With respect to a ``universe'' set $U$, we define the complement of $A$ as $U \smallsetminus A$, denoted $A^C$.
\end{definition}

The following hold:

\begin{itemize}
\item $(A \cup B)^C = A^C \cap B^C$
\item $(A \cap B)^C = A^C \cup B^C$
\end{itemize}

\paragraph{Cartesian product}

\begin{definition}
An \emph{ordered pair} is a set of the form $\lbrace \lbrace x \rbrace , \lbrace x, y \rbrace \rbrace$, denoted $(x, y)$ (where order matters).
\end{definition}

\begin{definition}
We define the \emph{cartesian product} $A\times B$ of two sets $A$ and $B$ as:

\begin{equation}
A\times B := \left\lbrace (a, b) : a \in A, b \in B \right\rbrace
\end{equation}
\end{definition}

\section{Propositional logic}

\paragraph{Implication}
\begin{definition}
\begin{equation}
p\implies q \iff (\neg p ) \vee q
\end{equation}
\end{definition}

\paragraph{Double implication}
\begin{definition}
\begin{equation}
(p \iff q) \iff (p \implies q \wedge q \implies p )
\end{equation}
\end{definition}

\paragraph{Quantifiers}

$P(x)$ is a \emph{predicate}. We say that $\forall x : P(x)$ if $P(x)$ is true independently of $x$, and that

\begin{equation}
\exists x : P(x) \iff \neg ( \forall x : \neg P(x) )
\end{equation}

\chapter{Number sets}

\section{The set $\mathbb{N}$}

\paragraph{The Peano axioms}

\begin{enumerate}
\item $1 \in \mathbb{N}$
\item $\forall n \in \mathbb{N}:  \exists S (n) : \mathbb{N} \rightarrow \mathbb{N}$
\item $\forall n \in \mathbb{N}: S(n) \neq 1$
\item $\forall m, n \in \mathbb{N}: m \neq n \implies S(n) \neq S(m)$ or $S(n) = S(m) \implies n = m$
\item $(A \subseteq \mathbb{N} )\wedge (1 \in A )\wedge (n  \in A \implies S(n) \in A ) \implies A = \mathbb{N}$
\end{enumerate}

Any set that verifies these axioms is isomorphic to $\mathbb{N}$. $\mathbb{R}^{+}$, for example only satisfies the first 4.

\section{Induction}

If $P(n)$ is a proposition, $P(1)$ and $P(n) \implies P(n+1)$\footnote{We introduce the notation $n+1$ to signify $S(n)$.} (the \emph{inductive hypothesis}); then $\forall n \in \mathbb{N}, P(n)$.

\begin{proof}
Define $A := \lbrace n \in \mathbb{N}: P(n) \rbrace$. By axiom 5, $A = \mathbb{N}$.
\end{proof}

If a property $a': P(k)$ holds for some $k \in \mathbb{N}$ and $b': P(n) \implies P(n+1)$, then $\forall n \geq k : P(n)$.

\paragraph{Examples}

Example: we can show by induction that

\begin{equation}
\sum_{i=1}^n = \frac{n (n+1)}{2}
\end{equation}

Example 2: we can show by induction that $P(\sharp A):\sharp \mathcal{P}(A) = 2^{\sharp A}$. 

\begin{proof}
$P(1)$ is true. 
We see that for any $A$ we can take an element such that $A = \lbrace a \rbrace \cup B$. Then for any subset $I$, either $a \in I$ or $a \not \in I$. If $a \in I$, $I = \lbrace a \rbrace \cup J$, but there are $2^n$ possible $J$s. If $a \not \in I$, we have $2^n$ $I'$s. So there are $2^{n+1}$ possible subsets.
\end{proof}

Example 3: show that $n! > 2^n$, which is true for $n>3$.

\begin{proof}
We will use the second form of the induction principle. $P(4)$ is true. If $n>4$ and $n! > 2^n$, we need to show that $(n+1) n!> 2 \cdot 2^n$. But $n+1>2$ by hypothesis, so the inequality always holds.
\end{proof}

Observation: the notation $1 + 2+ 3 + 4+ \cdots + n$ is unclear, we should use $\sum_{i=1}^n i$.

Recursive formulas: we know the first term, and an algorithm to derive any term from the one before it, such as the definition of the factorial:

\begin{equation}
\begin{cases}
0! = 1\\
(n+1)! = (n+1) n!
\end{cases}
\end{equation}

Another example is the sequence:

\begin{equation}
\begin{cases}
S_1 = 2\\
S_{n+1} = S_n + (2n+1)
\end{cases}
\end{equation}


\begin{proof}[Proof that $S_n = n^2 + 1$]
Assume that $S_n = n^2 +1$. Then $S_{n+1} = n^2 + 1 + 2n + 1 = (n+1)^2 + 1$.
\end{proof}

Formal definition of summation:

\begin{equation}
\sum_{i=0}^n a_i =a_0 + a_1 + a_2 + a_3 + \cdots + a_n
\end{equation}

by recursion: for an increment in $n$, we just add the $n+1$-th term. So it comes down to the formal definition of induction.

Example: show by induction that

\begin{equation}
\forall a \in \mathbb{N} \vee a=0 \quad (a\neq 1): \quad \sum_{k=0}^n a^k = \frac{1-a^{n+1}}{1-a}
\end{equation}

See the property for $n=0$. Suppose that the property holds for $n$, show it for $n+1$:

\begin{equation}
\sum_{i=0}^{n+1} a_k = \sum_{k=0}^n a^k + a^{n+1} = \frac{1-a^{n+1}}{1-a} + a^{n+1} = \frac{1-a^{n+2}}{1-a}
\end{equation}

To do: given two real numbers, $\forall n \in \mathbb{N}$, show that

\begin{equation}
(a+b)^n = \sum_{k=0}^n {n\choose k} a^k b^{n-k}
\end{equation}

\section{Groups}

We have a set $A$ with an operation $*$: $a, b \in A \rightarrow a*b \in A$. Es: $A$ strings, $*$ concatenation. $(A, *)$ is a group if the following are satisfied:

\begin{enumerate}
\item Associativity: $\forall a, b, c \in A: \quad a* (b*c) = (a*b)*c$
\item Identity: $\exists e \in A: \forall a \in A: \quad e*a = a*e = a$
\item Inverse: $\forall a \in A: \exists a^{-1} \in A: \quad a* a^{-1} = a^{-1} * a = e$
\end{enumerate}

$(A, *)$ is also a commutative group if $\forall a, b \in A: \quad a*b=b*a$

Examples: $(\mathbb{N}, +)$ is not a group: there is no identity, but even if we add 0 there is no inverse. $(\mathbb{Z}, +)$ is a commutative group. $(\mathbb{R}, \times)$ is not a group because 0 has no inverse. $(\mathbb{R}_0, \times)$ is hower a group, as is $(\mathbb{R}_0, +)$. $(\mathbb{Z}_0, \times)$ is not a group because there is no inverse: $(\mathbb{Q}_0, \times)$ is a commutative group.

So we introduce $\mathbb{Q}$:

\begin{equation}
\mathbb{Q}:= \left\lbrace \frac{a}{b}, a \in \mathbb{Z}, b\in \mathbb{N}\right\rbrace  / \sim
\end{equation}

but $ad \sim bc$ and $\mathbb{Q}$ is isomorphic to $\mathbb{Z}$

\begin{definition}
Order relation:

\begin{equation}
\frac a b \leq \frac cd \iff ad \leq bc 
\end{equation}
\end{definition}

\begin{definition}
Sum and product, subtraction and division are analogous:

\begin{equation}
\frac ab + \frac cd = \frac{ad+bc}{bd}
\end{equation}
\begin{equation}
\frac ab \times \frac cd = \frac{ac}{bd}
\end{equation}
\end{definition}

$(\mathbb{Q}, +, \times)$ is then a field:

\begin{enumerate}
\item $(\mathbb{Q}, +)$ is a commutative group;
\item $(\mathbb{Q}_0, \times )$ is a commutative group
\item $p (q+r) = pq + pr$
\end{enumerate}

\paragraph{Roots}

The square root of a number $a\geq 0$ is a $b \geq 0$ such that $b^2 = a$.

Show that in $\mathbb{Q}$ there is no $\sqrt{2}$:

\begin{proof}
By contradiction:\footnote{In the form: to show that $p \implies q$, we show that $\neg q \implies \neg p$, since
\begin{equation}
(p\implies q) \iff (\neg q \implies \neg p )
\end{equation}} if there were $a \in \mathbb{Z}$ and $b \in \mathbb{N}$ such that

\begin{equation}
\left( a\over b \right) ^2 = 2
\end{equation}

Suppose that $a, b$ have $\gcd(a, b) = 1$. Then $a^2 = 2 b^2$. So $a$ is even, and $a=2k$.

Then $4k^2 = 2b^2 \implies b=2n$: so $\gcd(a, b) \neq 1$
\end{proof}

To do: show that $\sqrt{3}$ is irrational, $\sqrt[3]{2}$ is irrational.

\section{The set $\mathbb{R}$}

The set is given.
$\mathbb{R}$ is a completely ordered field:

\begin{enumerate}
\item $(\mathbb{R}, +)$ is a commutative group
\item $(\mathbb{R}_0, \times)$ is a commutative group
\item $a (b+c) = ab+ac$
\end{enumerate}

There also exists a relation called $\leq$, such that $\forall a, b, c \in \mathbb{R}$:

\begin{enumerate}
\item $a\leq a$
\item $a \leq b \wedge b \leq a \implies a = b$
\item $a \leq b \wedge b \leq c \implies a \leq c$
\item $a \leq b \vee b \leq a$ (\emph{completely} ordered)
\item $a \leq b \implies a+c \leq b+c$
\item $a \geq 0 \wedge b \geq 0 \implies ab \geq 0$ (of course, $a \geq 0$ means that $0 \leq a$) 
\end{enumerate}

$(\mathbb{Q}, +, \times) $ is also a completely ordered field?

Take the set of all the real numbers whose squares are greater or equal to 2: it has a minimum.

In $\mathbb{Q}$, it has no minimum.

Other statements: show that $a \leq 0 \wedge b \geq 0 \implies ab \leq 0$

\begin{proof}
Is $a \geq 0 \wedge -b \geq 0$? We first need to show that $a \geq 0 \iff -a \leq 0$: it suffices to add $-a$ to both sides. We also need to show that $a (-b) = -ab$: by an inverse application of the distributive property.
\end{proof}

\tableofcontents

\end{document}
